rupicola/io/QExp.fst
@@ -111,13 +111,13 @@ and oprod_quotation : #a:qType -> g:typ_env -> fs_oprod g a -> Type =
         #g:typ_env ->
         #fnm:fs_oval g qBool ->
         oval_quotation g fnm ->
-        oprod_quotation #(qResexn qFileDescr) g (fs_oprod_openfile fnm)
+        oprod_quotation #(qResexn qFileDescr) g (fs_oprod_openfile_oval fnm)
 
 | QRead :
         #g:typ_env ->
         #fd:fs_oval g qFileDescr ->
         oval_quotation g fd ->
-        oprod_quotation #(qResexn qBool) g (fs_oprod_read fd)
+        oprod_quotation #(qResexn qBool) g (fs_oprod_read_oval fd)
 
 | QWrite :
         #g:typ_env ->
@@ -125,13 +125,13 @@ and oprod_quotation : #a:qType -> g:typ_env -> fs_oprod g a -> Type =
         #msg:fs_oval g qBool ->
         oval_quotation g fd ->
         oval_quotation g msg ->
-        oprod_quotation #(qResexn qUnit) g (fs_oprod_write fd msg)
+        oprod_quotation #(qResexn qUnit) g (fs_oprod_write_oval fd msg)
 
 | QClose :
         #g:typ_env ->
         #fd:fs_oval g qFileDescr ->
         oval_quotation g fd ->
-        oprod_quotation #(qResexn qUnit) g (fs_oprod_close fd)
+        oprod_quotation #(qResexn qUnit) g (fs_oprod_close_oval fd)
 
 | QReturn :
         #g:typ_env ->
